Define contexts, reduction and convertibility

theories/Constructions/Calculus.v
@@ -4,6 +4,7 @@
 
 Require Import Lia.
 Require Import Arith.
+Require Import Relations.
 Require Import Local.Prelude.
 Require Import Local.Substitution.
 Require Import Local.AbstractRewriting.
@@ -20,7 +21,7 @@ Inductive term: Set :=
   (* Products. *)
   | pi (t: term) (e: term)
   | abstraction (t: term) (e: term)
-  | application (f: term) (e: term)
+  | application (e: term) (f: term)
   | definition (e: term) (t: term) (f: term).
 
 Fixpoint traverse g k e: term :=
@@ -33,8 +34,8 @@ Fixpoint traverse g k e: term :=
     pi (traverse g k t) (traverse g (S k) e)
   | abstraction t e =>
     abstraction (traverse g k t) (traverse g (S k) e)
-  | application f e =>
-    application (traverse g k f) (traverse g k e)
+  | application e f =>
+    application (traverse g k e) (traverse g k f)
   | definition e t f =>
     definition (traverse g k e) (traverse g k t) (traverse g (S k) f)
   end.
@@ -89,3 +90,163 @@ Proof.
     induction x; simpl; intros; auto;
     f_equal; auto.
 Qed.
+
+Inductive context: Set :=
+  | context_hole
+  | context_pi_type (t: context) (e: term)
+  | context_pi_body (t: term) (e: context)
+  | context_abs_type (t: context) (e: term)
+  | context_abs_body (t: term) (e: context)
+  | context_app_left (f: context) (e: term)
+  | context_app_right (f: term) (e: context)
+  | context_def_val (e: context) (t: term) (f: term)
+  | context_def_type (e: term) (t: context) (f: term)
+  | context_def_body (e: term) (t: term) (f: context).
+
+Fixpoint apply_context (h: context) (x: term): term :=
+  match h with
+  | context_hole =>
+    x
+  | context_pi_type t e =>
+    pi (apply_context t x) e
+  | context_pi_body t e =>
+    pi t (apply_context e x)
+  | context_abs_type t e =>
+    abstraction (apply_context t x) e
+  | context_abs_body t e =>
+    abstraction t (apply_context e x)
+  | context_app_left f e =>
+    application (apply_context f x) e
+  | context_app_right f e =>
+    application f (apply_context e x)
+  | context_def_val e t f =>
+    definition (apply_context e x) t f
+  | context_def_type e t f =>
+    definition e (apply_context t x) f
+  | context_def_body e t f =>
+    definition e t (apply_context f x)
+  end.
+
+Coercion apply_context: context >-> Funclass.
+
+Inductive decl: Set :=
+  | decl_var (t: term)
+  | decl_def (e: term) (t: term).
+
+Definition env: Set :=
+  list decl.
+
+Inductive step (g: env): relation term :=
+  | step_beta:
+    forall t e f,
+    step g (application (abstraction t e) f) (subst f 0 e)
+  | step_zeta:
+    forall e t f,
+    step g (definition e t f) (subst e 0 f)
+  | step_delta:
+    forall t e n,
+    item (decl_def e t) g n ->
+    step g (bound n) (lift (S n) 0 e)
+  | step_pi_type:
+    forall t1 t2 e,
+    step g t1 t2 ->
+    step g (pi t1 e) (pi t2 e)
+  | step_pi_body:
+    forall t e1 e2,
+    step g e1 e2 ->
+    step g (pi t e1) (pi t e2)
+  | step_abs_type:
+    forall t1 t2 e,
+    step g t1 t2 ->
+    step g (abstraction t1 e) (abstraction t2 e)
+  | step_abs_body:
+    forall t e1 e2,
+    step g e1 e2 ->
+    step g (abstraction t e1) (abstraction t e2)
+  | step_app_left:
+    forall e1 e2 f,
+    step g e1 e2 ->
+    step g (application e1 f) (application e2 f)
+  | step_app_right:
+    forall e f1 f2,
+    step g f1 f2 ->
+    step g (application e f1) (application e f2)
+  | step_def_val:
+    forall e1 e2 t f,
+    step g e1 e2 ->
+    step g (definition e1 t f) (definition e2 t f)
+  | step_def_type:
+    forall e t1 t2 f,
+    step g t1 t2 ->
+    step g (definition e t1 f) (definition e t2 f)
+  | step_def_body:
+    forall e t f1 f2,
+    step g f1 f2 ->
+    step g (definition e t f1) (definition e t f2).
+
+Lemma step_context:
+  forall g e1 e2,
+  step g e1 e2 ->
+  forall h: context,
+  step g (h e1) (h e2).
+Proof.
+  induction h; simpl; intros.
+  - assumption.
+  - now constructor.
+  - now constructor.
+  - now constructor.
+  - now constructor.
+  - now constructor.
+  - now constructor.
+  - now constructor.
+  - now constructor.
+  - now constructor.
+Qed.
+
+Conjecture step_is_confluent: forall g, confluent (step g).
+
+Inductive conv: env -> relation term :=
+  | conv_join:
+    forall g e1 e2 f,
+    rt(step g) e1 f ->
+    rt(step g) e2 f ->
+    conv g e1 e2
+  | conv_eta_left:
+    forall g e1 e2 t f1 f2,
+    rt(step g) e1 (abstraction t f1) ->
+    rt(step g) e2 f2 ->
+    conv (decl_var t :: g) f1 (application f2 (bound 0)) ->
+    conv g e1 e2
+  | conv_eta_right:
+    forall g e1 e2 t f1 f2,
+    rt(step g) e1 f1 ->
+    rt(step g) e2 (abstraction t f2) ->
+    conv (decl_var t :: g) (application f1 (bound 0)) f2 ->
+    conv g e1 e2.
+
+Lemma conv_refl:
+  forall g,
+  reflexive (conv g).
+Proof.
+  repeat intro.
+  apply conv_join with x.
+  - apply rt_refl.
+  - apply rt_refl.
+Qed.
+
+Lemma conv_sym:
+  forall g,
+  symmetric (conv g).
+Proof.
+  induction 1.
+  - now apply conv_join with f.
+  - eapply conv_eta_right; eauto with cps.
+  - eapply conv_eta_left; eauto with cps.
+Qed.
+
+Lemma conv_trans:
+  forall g,
+  transitive (conv g).
+Proof.
+  admit.
+Admitted.
